
<!DOCTYPE rdf:RDF [
        <!ENTITY dc "http://purl.org/dc/" >
        <!ENTITY foaf "http://xmlns.com/foaf/0.1/" >
        <!ENTITY owl "http://www.w3.org/2002/07/owl#" >
        <!ENTITY xsd "http://www.w3.org/2001/XMLSchema#" >
        <!ENTITY prv "http://purl.org/ontology/prv/core#" >
        <!ENTITY rdfs "http://www.w3.org/2000/01/rdf-schema#" >
        <!ENTITY rdf "http://www.w3.org/1999/02/22-rdf-syntax-ns#" >
        <!ENTITY ms "http://metaservice.org/ns/metaservice#" >
        ]>

<rdf:RDF
        xml:base="http://metaservice.org/ns/metaservice#"
        xmlns:rdf="http://www.w3.org/1999/02/22-rdf-syntax-ns#"
        xmlns:rdfs="http://www.w3.org/2000/01/rdf-schema#"
        xmlns:owl="http://www.w3.org/2002/07/owl#"
        xmlns:vs="http://www.w3.org/2003/06/sw-vocab-status/ns#"
        xmlns:dc="http://purl.org/dc/"
        xmlns:vann="http://purl.org/vocab/vann/"
        xmlns:foaf="http://xmlns.com/foaf/spec/">
    <owl:Ontology rdf:about="&ms;">
        <dc:title>metaservice.org Metadata Ontology</dc:title>
        <dc:description>This ontology describes the Metadata structure in the metaservice.org database.</dc:description>
        <dc:creator>Nikola Ilo</dc:creator>
        <dc:format>application/rdf+xml</dc:format>
        <dc:rights>Copyright Â© 2013 Nikola Ilo</dc:rights>
        <vann:preferredNamespacePrefix>ms</vann:preferredNamespacePrefix>
        <vann:preferredNamespaceUri>http://metaservice.org/ns/metaservice#</vann:preferredNamespaceUri>
        <foaf:maker>
            <foaf:Person>
                <foaf:name>Nikola Ilo</foaf:name>
                <foaf:mbox rdf:resource="mailto:nikola.ilo@gmail.com"/>
            </foaf:Person>
        </foaf:maker>
    </owl:Ontology>

    <owl:Class rdf:about="&ms;Metadata" vs:term_status="unstable">
        <rdfs:label>Metadata</rdfs:label>
        <rdfs:comment>Named graph in the metaservice.org database.</rdfs:comment>
        <rdfs:isDefinedBy rdf:resource="&ms;"/>
    </owl:Class>

    <owl:DatatypeProperty rdf:about="&ms;action" vs:term_status="unstable" >
        <rdfs:label>action is</rdfs:label>
        <rdfs:comment>
            The Action denotes the operation.
            These operations determine the time scope on which the statements in the named graph are valid.
            Valid operations are "add", "remove" and continuous.
            A statement which was introduced in a graph which action was "add" is valid until there it occurs in a
            named graph with the action "remove".
            The semantics of "continuous" named graphs is as follows: All statements are valid as long as there is no
            named graph with a newer time and a subset or all same subject properties.
        </rdfs:comment>
        <rdfs:isDefinedBy rdf:resource="&ms;"/>
        <rdfs:domain rdf:resource="&ms;Metadata"/>
    </owl:DatatypeProperty>

    <owl:DatatypeProperty rdf:about="&ms;path" vs:term_status="unstable">
        <rdfs:label>originates from Path</rdfs:label>
        <rdfs:comment></rdfs:comment>
        <rdfs:isDefinedBy rdf:resource="&ms;"/>
        <rdfs:domain rdf:resource="&ms;Metadata"/>
    </owl:DatatypeProperty>

    <owl:DatatypeProperty rdf:about="&ms;time" vs:term_status="unstable">
        <rdfs:label>data source time</rdfs:label>
        <rdfs:comment>Time the described data was originally retrieved</rdfs:comment>
        <rdfs:isDefinedBy rdf:resource="&ms;"/>
        <rdfs:domain rdf:resource="&ms;Metadata"/>
    </owl:DatatypeProperty>

    <owl:DatatypeProperty rdf:about="&ms;generator" vs:term_status="unstable">
        <rdfs:label>generator of data</rdfs:label>
        <rdfs:comment>Identifier of the software which was used to create the statements.</rdfs:comment>
        <rdfs:isDefinedBy rdf:resource="&ms;"/>
        <rdfs:domain rdf:resource="&ms;Metadata"/>
    </owl:DatatypeProperty>

    <owl:DatatypeProperty rdf:about="&ms;creationTime" vs:term_status="unstable">
        <rdfs:label>created on</rdfs:label>
        <rdfs:comment>The time this set of changes where created.</rdfs:comment>
        <rdfs:isDefinedBy rdf:resource="&ms;"/>
        <rdfs:domain rdf:resource="&ms;Metadata"/>
    </owl:DatatypeProperty>

    <owl:DatatypeProperty rdf:about="&ms;lastCheckedTime" vs:term_status="unstable">
        <rdfs:label>last checked on</rdfs:label>
        <rdfs:comment>The last time the set of statements where checked for changes and found unchanged.</rdfs:comment>
        <rdfs:isDefinedBy rdf:resource="&ms;"/>
        <rdfs:domain rdf:resource="&ms;Metadata"/>
    </owl:DatatypeProperty>

    <owl:DatatypeProperty rdf:about="&ms;source" vs:term_status="unstable">
        <rdfs:label>retrieved from</rdfs:label>
        <rdfs:comment>uri of the archive, where the statements were retrieved from</rdfs:comment>
        <rdfs:isDefinedBy rdf:resource="&ms;"/>
        <rdfs:domain rdf:resource="&ms;Metadata"/>
    </owl:DatatypeProperty>

    <owl:DatatypeProperty rdf:about="&ms;repositoryId" vs:term_status="unstable">
        <rdfs:label>repository</rdfs:label>
        <rdfs:comment>id of the repository this was retrieved from</rdfs:comment>
        <rdfs:isDefinedBy rdf:resource="&ms;"/>
        <rdfs:domain rdf:resource="&ms;Metadata"/>
    </owl:DatatypeProperty>


    <owl:DatatypeProperty rdf:about="&ms;latest" vs:term_status="unstable">
        <rdfs:label>valid on date</rdfs:label>
        <rdfs:comment>valid for postprocessors. Calculated validity of the statements for the given date.</rdfs:comment>
        <rdfs:isDefinedBy rdf:resource="&ms;"/>
        <rdfs:domain rdf:resource="&ms;Metadata"/>
    </owl:DatatypeProperty>

    <owl:DatatypeProperty rdf:about="&ms;view" vs:term_status="unstable">
        <rdfs:label>displayable by template</rdfs:label>
        <rdfs:comment>Links a class to a metaservice.org template</rdfs:comment>
        <rdfs:isDefinedBy rdf:resource="&ms;"/>
        <rdfs:domain rdf:resource="&rdfs;Class"/>
    </owl:DatatypeProperty>

    <owl:ObjectProperty rdf:about="&ms;sourceSubject" vs:term_status="unstable">
        <rdfs:label>produced from</rdfs:label>
        <rdfs:comment>Resources which are processed together and are important for the time validity scope of the
            named graph</rdfs:comment>
        <rdfs:isDefinedBy rdf:resource="&ms;"/>
    </owl:ObjectProperty>


    <owl:ObjectProperty rdf:about="&ms;dummy" vs:term_status="unstable">
        <rdfs:label>Dummy Statement</rdfs:label>
        <rdfs:comment>A dummy statement - used internally to denote empty results</rdfs:comment>
        <rdfs:isDefinedBy rdf:resource="&ms;"/>
    </owl:ObjectProperty>


    <owl:NamedIndividual rdf:about="&ms;ActionAdd">
        <rdf:type rdf:resource="&owl;Thing"/>
        <rdfs:label>Add</rdfs:label>
        <rdfs:comment>Introduce Statements</rdfs:comment>
        <rdfs:isDefinedBy rdf:resource="&ms;"/>
    </owl:NamedIndividual>

    <owl:NamedIndividual rdf:about="&ms;ActionRemove">
        <rdf:type rdf:resource="&owl;Thing"/>
        <rdfs:label>Add</rdfs:label>
        <rdfs:comment>Remove Statements</rdfs:comment>
        <rdfs:isDefinedBy rdf:resource="&ms;"/>
    </owl:NamedIndividual>

    <owl:NamedIndividual rdf:about="&ms;ActionContinuous">
        <rdf:type rdf:resource="&owl;Thing"/>
        <rdfs:label>Continuous</rdfs:label>
        <rdfs:comment>Introduce continuous Statements, which are valid until it is stated otherwise.</rdfs:comment>
        <rdfs:isDefinedBy rdf:resource="&ms;"/>
    </owl:NamedIndividual>


</rdf:RDF>